update

theory/Sound_Framework.thy
@@ -4,72 +4,107 @@ theory Sound_Framework
       "~~/src/HOL/Eisbach/Eisbach_Tools"
 begin
 
-inductive is_super_stack :: "cont list \<Rightarrow> exp \<Rightarrow> bool" where
-  Exp: "
-    is_super_exp e e' \<Longrightarrow>
-    is_super_stack (\<langle>x, e, \<rho>\<rangle> # \<kappa>) e'
+inductive is_super_exp_over_stack :: "exp \<Rightarrow> cont list \<Rightarrow> bool" where
+  Empty: "
+    is_super_exp_over_stack e0 []
   " |
-  Stack: "
-    is_super_stack \<kappa> e' \<Longrightarrow>
-    is_super_stack (\<langle>x, e, \<rho>\<rangle> # \<kappa>) e'
+  Nonempty: "
+    is_super_exp_left e0 e\<^sub>\<kappa> \<Longrightarrow>
+    (* is_super_exp_over_stack e0 \<kappa> \<Longrightarrow> *)
+    is_super_exp_over_stack e0 (\<langle>x\<^sub>\<kappa>,e\<^sub>\<kappa>,\<rho>\<^sub>\<kappa>\<rangle> # \<kappa>)
+  "
+
+inductive is_super_exp_over_state :: "exp \<Rightarrow> state \<Rightarrow> bool" where
+  "
+    is_super_exp_left e0 e \<Longrightarrow>
+    is_super_exp_over_stack e0 \<kappa> \<Longrightarrow>
+    is_super_exp_over_state e0 (\<langle>e;\<rho>;\<kappa>\<rangle>)
   "
 
 lemma is_super_exp_preserved: "
   E \<rightarrow> E' \<Longrightarrow>
-  \<forall>\<pi> e \<rho> \<kappa>. E \<pi> = Some (\<langle>e;\<rho>;\<kappa>\<rangle>) \<longrightarrow> is_super_exp e\<^sub>0 e \<Longrightarrow>
-  E' \<pi>' = Some (\<langle>e';\<rho>';\<kappa>'\<rangle>) \<Longrightarrow>
-  is_super_exp_left e\<^sub>0 e'
+  \<forall>\<pi> \<sigma>. E \<pi> = Some \<sigma> \<longrightarrow> is_super_exp_over_state e\<^sub>0 \<sigma> \<Longrightarrow>
+  E' \<pi>' = Some \<sigma>' \<Longrightarrow>
+  is_super_exp_over_state e\<^sub>0 \<sigma>'
 "
-sorry
+proof -
+
+  assume 
+    A: "\<forall>\<pi> \<sigma>. E \<pi> = Some \<sigma> \<longrightarrow> is_super_exp_over_state e\<^sub>0 \<sigma>" and
+    B: "E' \<pi>' = Some \<sigma>'"
+
+  assume "E \<rightarrow> E'" then
+
+  show "  is_super_exp_over_state e\<^sub>0 \<sigma>'" 
+  proof cases
+    case (Seq_Step_Down \<pi> x \<rho> x\<^sub>\<kappa> e\<^sub>\<kappa> \<rho>\<^sub>\<kappa> \<kappa> \<sigma>')
+    then show ?thesis sorry
+  next
+    case (Seq_Step \<pi> x b e \<rho> \<kappa> e' \<rho>')
+    then show ?thesis sorry
+  next
+    case (Seq_Step_Up \<pi> x b e \<rho> \<kappa> e' \<rho>')
+    then show ?thesis sorry
+  next
+    case (Let_Chan \<pi> x e \<rho> \<kappa>)
+    then show ?thesis sorry
+  next
+    case (Let_Spawn \<pi> x e\<^sub>c e \<rho> \<kappa>)
+    then show ?thesis sorry
+  next
+    case (Let_Sync \<pi>\<^sub>s x\<^sub>s x\<^sub>s\<^sub>e e\<^sub>s \<rho>\<^sub>s \<kappa>\<^sub>s x\<^sub>s\<^sub>c x\<^sub>m \<rho>\<^sub>s\<^sub>e \<pi>\<^sub>r x\<^sub>r x\<^sub>r\<^sub>e e\<^sub>r \<rho>\<^sub>r \<kappa>\<^sub>r x\<^sub>r\<^sub>c \<rho>\<^sub>r\<^sub>e c \<omega>\<^sub>m)
+    then show ?thesis sorry
+  qed
+qed
 
 
 lemma isnt_exp_sound_generalized: "
   \<E>0 \<rightarrow>* \<E>' \<Longrightarrow>
   \<E>0 = [[] \<mapsto> \<langle>e\<^sub>0;Map.empty;[]\<rangle>] \<Longrightarrow>
-  \<E>' \<pi>' = Some (\<langle>e';\<rho>';\<kappa>'\<rangle>) \<Longrightarrow>
-  is_super_exp e\<^sub>0 e'
+  \<E>' \<pi>' = Some \<sigma>' \<Longrightarrow>
+  is_super_exp_over_state e\<^sub>0 \<sigma>'
 "
 proof -
 
-  assume P1: "\<E>0 = [[] \<mapsto> \<langle>e\<^sub>0;Map.empty;[]\<rangle>]" and P2: "\<E>' \<pi>' = Some (\<langle>e';\<rho>';\<kappa>'\<rangle>)"
+  assume P1: "\<E>0 = [[] \<mapsto> \<langle>e\<^sub>0;Map.empty;[]\<rangle>]" and P2: "\<E>' \<pi>' = Some \<sigma>'"
 
   assume "\<E>0 \<rightarrow>* \<E>'" then
 
   have "star_left (op \<rightarrow>) \<E>0 \<E>'" by (simp add: star_implies_star_left) then
 
   have "
-    \<forall> \<pi>' e' \<rho>' \<kappa>' .
+    \<forall> \<pi>' \<sigma>' .
     \<E>0 = [[] \<mapsto> \<langle>e\<^sub>0;Map.empty;[]\<rangle>] \<longrightarrow>
-    \<E>' \<pi>' = Some (\<langle>e';\<rho>';\<kappa>'\<rangle>) \<longrightarrow>
-    is_super_exp e\<^sub>0 e'
+    \<E>' \<pi>' = Some \<sigma>' \<longrightarrow>
+    is_super_exp_over_state e\<^sub>0 \<sigma>'
   " proof (induction)
     case (refl x)
-    show ?case by (simp add: is_super_exp.Refl)
+    show ?case by (simp add: is_super_exp_left.Refl is_super_exp_over_stack.Empty is_super_exp_over_state.intros)
   next
     case (step E0 E E')
     assume "star_left op \<rightarrow> E0 E"
     assume "E \<rightarrow> E'"
-    assume IH: "\<forall>\<pi>' e' \<rho>' \<kappa>'. E0 = [[] \<mapsto> \<langle>e\<^sub>0;Map.empty;[]\<rangle>] \<longrightarrow> E \<pi>' = Some (\<langle>e';\<rho>';\<kappa>'\<rangle>) \<longrightarrow> is_super_exp e\<^sub>0 e'"
+    assume IH: "\<forall>\<pi>' \<sigma>'. E0 = [[] \<mapsto> \<langle>e\<^sub>0;Map.empty;[]\<rangle>] \<longrightarrow> E \<pi>' = Some \<sigma>' \<longrightarrow> is_super_exp_over_state e\<^sub>0 \<sigma>'"
     {
-      fix \<pi>' e' \<rho>' \<kappa>'
+      fix \<pi>' \<sigma>'
       assume 
         P1: "E0 = [[] \<mapsto> \<langle>e\<^sub>0;Map.empty;[]\<rangle>]" and
-        P2: "E' \<pi>' = Some (\<langle>e';\<rho>';\<kappa>'\<rangle>)" 
+        P2: "E' \<pi>' = Some \<sigma>'" 
 
       from IH and P1
 
-      have IH2: "\<forall>\<pi>' e' \<rho>' \<kappa>'. E \<pi>' = Some (\<langle>e';\<rho>';\<kappa>'\<rangle>) \<longrightarrow> is_super_exp e\<^sub>0 e'" by blast
+      have IH2: "\<forall>\<pi>' \<sigma>'. E \<pi>' = Some \<sigma>' \<longrightarrow> is_super_exp_over_state e\<^sub>0 \<sigma>'"  by blast
       with P2 \<open>E \<rightarrow> E'\<close>
 
-      have "is_super_exp_left e\<^sub>0 e'" by (blast dest: is_super_exp_preserved) then
+      have "is_super_exp_over_state e\<^sub>0 \<sigma>'" by (blast dest: is_super_exp_preserved) then
 
-      have "is_super_exp e\<^sub>0 e'" by (simp add: is_super_exp_left_implies_is_super_exp)
+      have "is_super_exp_over_state e\<^sub>0 \<sigma>'" by (simp add: is_super_exp_left_implies_is_super_exp)
     } then
     show ?case by blast
   qed
   with P1 and P2
 
-  show "is_super_exp e\<^sub>0 e'"  by blast
+  show "is_super_exp_over_state e\<^sub>0 \<sigma>'" by blast
 qed
 
 lemma isnt_exp_sound: "
@@ -77,7 +112,7 @@ lemma isnt_exp_sound: "
   \<E>' \<pi>' = Some (\<langle>e';\<rho>';\<kappa>'\<rangle>) \<Longrightarrow>
   is_super_exp e\<^sub>0 e'
 "
-sorry
+by (metis is_super_exp_left_implies_is_super_exp is_super_exp_over_state.cases isnt_exp_sound_generalized state.inject)
 
 
 end
